src/MemoryOps.v
@@ -15,165 +15,108 @@ Inductive loc : Set :=
 
 Section GPR.
 (** Fetching value from general purpose register. *)
-Inductive fetch_gpr : regs_state -> reg_name -> primitive_value -> Prop :=
-| fr_fetch0:
-  forall regs,
-    fetch_gpr regs R0 (IntValue zero256)
-| fr_fetch1:
-  forall r0 r1 r2 r3 r4 r5 r6 r7 r8 r9 r10 r11 r12 r13 r14 r15,
-    fetch_gpr (mk_regs [r0; r1; r2; r3; r4; r5; r6; r7; r8; r9; r10 ; r11; r12
-                        ; r13; r14; r15])
-      R1 r1
-| fr_fetch2:
-  forall r0 r1 r2 r3 r4 r5 r6 r7 r8 r9 r10 r11 r12 r13 r14 r15,
-    fetch_gpr (mk_regs [r0; r1; r2; r3; r4; r5; r6; r7; r8; r9; r10 ; r11; r12
-                        ; r13; r14; r15])
-      R2 r2
-| fr_fetch3:
-  forall r0 r1 r2 r3 r4 r5 r6 r7 r8 r9 r10 r11 r12 r13 r14 r15,
-    fetch_gpr (mk_regs [r0; r1; r2; r3; r4; r5; r6; r7; r8; r9; r10 ; r11; r12
-                        ; r13; r14; r15])
-      R3 r3
-| fr_fetch4:
-  forall r0 r1 r2 r3 r4 r5 r6 r7 r8 r9 r10 r11 r12 r13 r14 r15,
-    fetch_gpr (mk_regs [r0; r1; r2; r3; r4; r5; r6; r7; r8; r9; r10 ; r11; r12
-                        ; r13; r14; r15])
-      R4 r4
-| fr_fetch5:
-  forall r0 r1 r2 r3 r4 r5 r6 r7 r8 r9 r10 r11 r12 r13 r14 r15,
-    fetch_gpr (mk_regs [r0; r1; r2; r3; r4; r5; r6; r7; r8; r9; r10 ; r11; r12
-                        ; r13; r14; r15])
-      R5 r5
-| fr_fetch6:
-  forall r0 r1 r2 r3 r4 r5 r6 r7 r8 r9 r10 r11 r12 r13 r14 r15,
-    fetch_gpr (mk_regs [r0; r1; r2; r3; r4; r5; r6; r7; r8; r9; r10 ; r11; r12
-                        ; r13; r14; r15])
-      R6 r6
-| fr_fetch7:
-  forall r0 r1 r2 r3 r4 r5 r6 r7 r8 r9 r10 r11 r12 r13 r14 r15,
-    fetch_gpr (mk_regs [r0; r1; r2; r3; r4; r5; r6; r7; r8; r9; r10 ; r11; r12
-                        ; r13; r14; r15])
-      R7 r7
-| fr_fetch8:
-  forall r0 r1 r2 r3 r4 r5 r6 r7 r8 r9 r10 r11 r12 r13 r14 r15,
-    fetch_gpr (mk_regs [r0; r1; r2; r3; r4; r5; r6; r7; r8; r9; r10 ; r11; r12
-                        ; r13; r14; r15])
-      R8 r8
-| fr_fetch9:
-  forall r0 r1 r2 r3 r4 r5 r6 r7 r8 r9 r10 r11 r12 r13 r14 r15,
-    fetch_gpr (mk_regs [r0; r1; r2; r3; r4; r5; r6; r7; r8; r9; r10 ; r11; r12
-                        ; r13; r14; r15])
-      R9 r9
-| fr_fetch10:
-  forall r0 r1 r2 r3 r4 r5 r6 r7 r8 r9 r10 r11 r12 r13 r14 r15,
-    fetch_gpr (mk_regs [r0; r1; r2; r3; r4; r5; r6; r7; r8; r9; r10 ; r11; r12
-                        ; r13; r14; r15])
-      R10 r10
-| fr_fetch11:
-  forall r0 r1 r2 r3 r4 r5 r6 r7 r8 r9 r10 r11 r12 r13 r14 r15,
-    fetch_gpr (mk_regs [r0; r1; r2; r3; r4; r5; r6; r7; r8; r9; r10 ; r11; r12
-                        ; r13; r14; r15])
-      R11 r11
-| fr_fetch12:
-  forall r0 r1 r2 r3 r4 r5 r6 r7 r8 r9 r10 r11 r12 r13 r14 r15,
-    fetch_gpr (mk_regs [r0; r1; r2; r3; r4; r5; r6; r7; r8; r9; r10 ; r11; r12
-                        ; r13; r14; r15])
-      R12 r12
-| fr_fetch13:
-  forall r0 r1 r2 r3 r4 r5 r6 r7 r8 r9 r10 r11 r12 r13 r14 r15,
-    fetch_gpr (mk_regs [r0; r1; r2; r3; r4; r5; r6; r7; r8; r9; r10 ; r11; r12
-                        ; r13; r14; r15])
-      R13 r13
-| fr_fetch14:
-  forall r0 r1 r2 r3 r4 r5 r6 r7 r8 r9 r10 r11 r12 r13 r14 r15,
-    fetch_gpr (mk_regs [r0; r1; r2; r3; r4; r5; r6; r7; r8; r9; r10 ; r11; r12
-                        ; r13; r14; r15])
-      R14 r14
-| fr_fetch15:
-  forall r0 r1 r2 r3 r4 r5 r6 r7 r8 r9 r10 r11 r12 r13 r14 r15,
-    fetch_gpr (mk_regs [r0; r1; r2; r3; r4; r5; r6; r7; r8; r9; r10 ; r11; r12
-                        ; r13; r14; r15])
-      R15 r15
-.
+
+  Definition fetch_gpr (rs:regs_state) (r:reg_name) : primitive_value :=
+    match r with
+    | R0 => IntValue zero256
+    | R1 => gprs_r1 rs
+    | R2 => gprs_r2 rs
+    | R3 => gprs_r3 rs
+    | R4 => gprs_r4 rs
+    | R5 => gprs_r5 rs
+    | R6 => gprs_r6 rs
+    | R7 => gprs_r7 rs
+    | R8 => gprs_r8 rs
+    | R9 => gprs_r9 rs
+    | R10 => gprs_r10 rs
+    | R11 => gprs_r11 rs
+    | R12 => gprs_r12 rs
+    | R13 => gprs_r13 rs
+    | R14 => gprs_r14 rs
+    | R15 => gprs_r15 rs
+    end.
+
+(** Storing value to general purpose registers. *)
+
+
 
 (** Storing value to general purpose registers. *)
 Inductive store_gpr : regs_state -> reg_name -> primitive_value -> regs_state -> Prop :=
 | fr_store1 :
-  forall r0 r1 r2 r3 r4 r5 r6 r7 r8 r9 r10 r11 r12 r13 r14 r15 pv,
-  store_gpr (mk_regs [r0; r1; r2; r3; r4; r5; r6; r7; r8; r9; r10
-                      ; r11; r12; r13; r14; r15]) R1 pv (mk_regs [r0; pv; r2; r3; r4; r5; r6; r7; r8; r9; r10
-                      ; r11; r12; r13; r14; r15])
+  forall r1 r2 r3 r4 r5 r6 r7 r8 r9 r10 r11 r12 r13 r14 r15 pv,
+  store_gpr
+    (mk_regs r1 r2 r3 r4 r5 r6 r7 r8 r9 r10 r11 r12 r13 r14 r15) R1 pv
+    (mk_regs pv r2 r3 r4 r5 r6 r7 r8 r9 r10 r11 r12 r13 r14 r15)
 | fr_store2 :
-  forall r0 r1 r2 r3 r4 r5 r6 r7 r8 r9 r10 r11 r12 r13 r14 r15 pv,
-  store_gpr (mk_regs [r0; r1; r2; r3; r4; r5; r6; r7; r8; r9; r10
-                      ; r11; r12; r13; r14; r15]) R2 pv (mk_regs [r0; r1; pv; r3; r4; r5; r6; r7; r8; r9; r10
-                      ; r11; r12; r13; r14; r15])
+  forall r1 r2 r3 r4 r5 r6 r7 r8 r9 r10 r11 r12 r13 r14 r15 pv,
+  store_gpr
+    (mk_regs r1 r2 r3 r4 r5 r6 r7 r8 r9 r10 r11 r12 r13 r14 r15) R2 pv
+    (mk_regs r1 pv r3 r4 r5 r6 r7 r8 r9 r10 r11 r12 r13 r14 r15)
 | fr_store3 :
-  forall r0 r1 r2 r3 r4 r5 r6 r7 r8 r9 r10 r11 r12 r13 r14 r15 pv,
-  store_gpr (mk_regs [r0; r1; r2; r3; r4; r5; r6; r7; r8; r9; r10
-                      ; r11; r12; r13; r14; r15]) R3 pv (mk_regs [r0; r1; r2; pv; r4; r5; r6; r7; r8; r9; r10
-                      ; r11; r12; r13; r14; r15])
+  forall r1 r2 r3 r4 r5 r6 r7 r8 r9 r10 r11 r12 r13 r14 r15 pv,
+  store_gpr
+    (mk_regs r1 r2 r3 r4 r5 r6 r7 r8 r9 r10 r11 r12 r13 r14 r15) R3 pv
+    (mk_regs r1 r2 pv r4 r5 r6 r7 r8 r9 r10 r11 r12 r13 r14 r15)
 | fr_store4 :
-  forall r0 r1 r2 r3 r4 r5 r6 r7 r8 r9 r10 r11 r12 r13 r14 r15 pv,
-  store_gpr (mk_regs [r0; r1; r2; r3; r4; r5; r6; r7; r8; r9; r10
-                      ; r11; r12; r13; r14; r15]) R4 pv (mk_regs [r0; r1; r2; r3; pv; r5; r6; r7; r8; r9; r10
-                      ; r11; r12; r13; r14; r15])
+  forall r1 r2 r3 r4 r5 r6 r7 r8 r9 r10 r11 r12 r13 r14 r15 pv,
+  store_gpr
+    (mk_regs r1 r2 r3 r4 r5 r6 r7 r8 r9 r10 r11 r12 r13 r14 r15) R4 pv
+    (mk_regs r1 r2 r3 pv r5 r6 r7 r8 r9 r10 r11 r12 r13 r14 r15)
 | fr_store5 :
-  forall r0 r1 r2 r3 r4 r5 r6 r7 r8 r9 r10 r11 r12 r13 r14 r15 pv,
-  store_gpr (mk_regs [r0; r1; r2; r3; r4; r5; r6; r7; r8; r9; r10
-                      ; r11; r12; r13; r14; r15]) R5 pv (mk_regs [r0; r1; r2; r3; r4; pv; r6; r7; r8; r9; r10
-                      ; r11; r12; r13; r14; r15])
+  forall r1 r2 r3 r4 r5 r6 r7 r8 r9 r10 r11 r12 r13 r14 r15 pv,
+  store_gpr
+    (mk_regs r1 r2 r3 r4 r5 r6 r7 r8 r9 r10 r11 r12 r13 r14 r15) R5 pv
+    (mk_regs r1 r2 r3 r4 pv r6 r7 r8 r9 r10 r11 r12 r13 r14 r15)
 | fr_store6 :
-  forall r0 r1 r2 r3 r4 r5 r6 r7 r8 r9 r10 r11 r12 r13 r14 r15 pv,
-  store_gpr (mk_regs [r0; r1; r2; r3; r4; r5; r6; r7; r8; r9; r10
-                      ; r11; r12; r13; r14; r15]) R6 pv (mk_regs [r0; r1; r2; r3; r4; r5; pv; r7; r8; r9; r10
-                      ; r11; r12; r13; r14; r15])
+  forall r1 r2 r3 r4 r5 r6 r7 r8 r9 r10 r11 r12 r13 r14 r15 pv,
+    store_gpr
+      (mk_regs r1 r2 r3 r4 r5 r6 r7 r8 r9 r10 r11 r12 r13 r14 r15) R6 pv
+      (mk_regs r1 r2 r3 r4 r5 pv r7 r8 r9 r10 r11 r12 r13 r14 r15)
 | fr_store7 :
-  forall r0 r1 r2 r3 r4 r5 r6 r7 r8 r9 r10 r11 r12 r13 r14 r15 pv,
-  store_gpr (mk_regs [r0; r1; r2; r3; r4; r5; r6; r7; r8; r9; r10
-                      ; r11; r12; r13; r14; r15]) R7 pv (mk_regs [r0; r1; r2; r3; r4; r5; r6; pv; r8; r9; r10
-                      ; r11; r12; r13; r14; r15])
+  forall r1 r2 r3 r4 r5 r6 r7 r8 r9 r10 r11 r12 r13 r14 r15 pv,
+    store_gpr
+      (mk_regs r1 r2 r3 r4 r5 r6 r7 r8 r9 r10 r11 r12 r13 r14 r15) R7 pv
+      (mk_regs r1 r2 r3 r4 r5 r6 pv r8 r9 r10 r11 r12 r13 r14 r15)
 | fr_store8 :
-  forall r0 r1 r2 r3 r4 r5 r6 r7 r8 r9 r10 r11 r12 r13 r14 r15 pv,
-  store_gpr (mk_regs [r0; r1; r2; r3; r4; r5; r6; r7; r8; r9; r10
-                      ; r11; r12; r13; r14; r15]) R8 pv (mk_regs [r0; r1; r2; r3; r4; r5; r6; r7; pv; r9; r10
-                      ; r11; r12; r13; r14; r15])
+  forall r1 r2 r3 r4 r5 r6 r7 r8 r9 r10 r11 r12 r13 r14 r15 pv,
+    store_gpr
+      (mk_regs r1 r2 r3 r4 r5 r6 r7 r8 r9 r10 r11 r12 r13 r14 r15) R8 pv
+      (mk_regs r1 r2 r3 r4 r5 r6 r7 pv r9 r10 r11 r12 r13 r14 r15)
 | fr_store9 :
-  forall r0 r1 r2 r3 r4 r5 r6 r7 r8 r9 r10 r11 r12 r13 r14 r15 pv,
-  store_gpr (mk_regs [r0; r1; r2; r3; r4; r5; r6; r7; r8; r9; r10
-                      ; r11; r12; r13; r14; r15]) R9 pv (mk_regs [r0; r1; r2; r3; r4; r5; r6; r7; r8; pv; r10
-                      ; r11; r12; r13; r14; r15])
+  forall r1 r2 r3 r4 r5 r6 r7 r8 r9 r10 r11 r12 r13 r14 r15 pv,
+    store_gpr
+      (mk_regs r1 r2 r3 r4 r5 r6 r7 r8 r9 r10 r11 r12 r13 r14 r15) R9 pv
+      (mk_regs r1 r2 r3 r4 r5 r6 r7 r8 pv r10 r11 r12 r13 r14 r15)
 | fr_store10 :
-  forall r0 r1 r2 r3 r4 r5 r6 r7 r8 r9 r10 r11 r12 r13 r14 r15 pv,
-  store_gpr (mk_regs [r0; r1; r2; r3; r4; r5; r6; r7; r8; r9; r10
-                      ; r11; r12; r13; r14; r15]) R10 pv
-    (mk_regs [r0; r1; r2; r3; r4; r5; r6; r7; r8; r9; pv 
-                      ; r11; r12; r13; r14; r15])
+  forall r1 r2 r3 r4 r5 r6 r7 r8 r9 r10 r11 r12 r13 r14 r15 pv,
+    store_gpr
+      (mk_regs r1 r2 r3 r4 r5 r6 r7 r8 r9 r10 r11 r12 r13 r14 r15) R10 pv
+      (mk_regs r1 r2 r3 r4 r5 r6 r7 r8 r9 pv r11 r12 r13 r14 r15)
 | fr_store11 :
-  forall r0 r1 r2 r3 r4 r5 r6 r7 r8 r9 r10 r11 r12 r13 r14 r15 pv,
-  store_gpr (mk_regs [r0; r1; r2; r3; r4; r5; r6; r7; r8; r9; r10
-                      ; r11; r12; r13; r14; r15]) R11 pv (mk_regs [r0; r1; r2; r3; r4; r5; r6; r7; r8; r9; r10
-                      ; pv; r12; r13; r14; r15])
+  forall r1 r2 r3 r4 r5 r6 r7 r8 r9 r10 r11 r12 r13 r14 r15 pv,
+    store_gpr
+      (mk_regs r1 r2 r3 r4 r5 r6 r7 r8 r9 r10 r11 r12 r13 r14 r15) R11 pv
+      (mk_regs r1 r2 r3 r4 r5 r6 r7 r8 r9 r10 pv r12 r13 r14 r15)
 | fr_store12 :
-  forall r0 r1 r2 r3 r4 r5 r6 r7 r8 r9 r10 r11 r12 r13 r14 r15 pv,
-  store_gpr (mk_regs [r0; r1; r2; r3; r4; r5; r6; r7; r8; r9; r10
-                      ; r11; r12; r13; r14; r15]) R12 pv (mk_regs [r0; r1; r2; r3; r4; r5; r6; r7; r8; r9; r10
-                      ; r11; pv; r13; r14; r15])
+  forall r1 r2 r3 r4 r5 r6 r7 r8 r9 r10 r11 r12 r13 r14 r15 pv,
+    store_gpr
+      (mk_regs r1 r2 r3 r4 r5 r6 r7 r8 r9 r10 r11 r12 r13 r14 r15) R12 pv
+      (mk_regs r1 r2 r3 r4 r5 r6 r7 r8 r9 r10 r11 pv r13 r14 r15)
 | fr_store13 :
-  forall r0 r1 r2 r3 r4 r5 r6 r7 r8 r9 r10 r11 r12 r13 r14 r15 pv,
-  store_gpr (mk_regs [r0; r1; r2; r3; r4; r5; r6; r7; r8; r9; r10
-                      ; r11; r12; r13; r14; r15]) R13 pv (mk_regs [r0; r1; r2; r3; r4; r5; r6; r7; r8; r9; r10
-                      ; r11; r12; pv; r14; r15])
+  forall r1 r2 r3 r4 r5 r6 r7 r8 r9 r10 r11 r12 r13 r14 r15 pv,
+    store_gpr
+      (mk_regs r1 r2 r3 r4 r5 r6 r7 r8 r9 r10 r11 r12 r13 r14 r15) R13 pv
+      (mk_regs r1 r2 r3 r4 r5 r6 r7 r8 r9 r10 r11 r12 pv r14 r15)
 | fr_store14 :
-  forall r0 r1 r2 r3 r4 r5 r6 r7 r8 r9 r10 r11 r12 r13 r14 r15 pv,
-  store_gpr (mk_regs [r0; r1; r2; r3; r4; r5; r6; r7; r8; r9; r10
-                      ; r11; r12; r13; r14; r15]) R14 pv (mk_regs [r0; r1; r2; r3; r4; r5; r6; r7; r8; r9; r10
-                      ; r11; r12; r13; pv; r15])
+  forall r1 r2 r3 r4 r5 r6 r7 r8 r9 r10 r11 r12 r13 r14 r15 pv,
+    store_gpr
+      (mk_regs r1 r2 r3 r4 r5 r6 r7 r8 r9 r10 r11 r12 r13 r14 r15) R14 pv
+      (mk_regs r1 r2 r3 r4 r5 r6 r7 r8 r9 r10 r11 r12 r13 pv r15)
 | fr_store15 :
-  forall r0 r1 r2 r3 r4 r5 r6 r7 r8 r9 r10 r11 r12 r13 r14 r15 pv,
-  store_gpr (mk_regs [r0; r1; r2; r3; r4; r5; r6; r7; r8; r9; r10
-                      ; r11; r12; r13; r14; r15]) R15 pv (mk_regs [r0; r1; r2; r3; r4; r5; r6; r7; r8; r9; r10
-                      ; r11; r12; r13; r14; pv])
+  forall r1 r2 r3 r4 r5 r6 r7 r8 r9 r10 r11 r12 r13 r14 r15 pv,
+    store_gpr
+      (mk_regs r1 r2 r3 r4 r5 r6 r7 r8 r9 r10 r11 r12 r13 r14 r15) R15 pv
+      (mk_regs r1 r2 r3 r4 r5 r6 r7 r8 r9 r10 r11 r12 r13 r14 pv)
 .
 
 End GPR.
@@ -183,7 +126,7 @@ Section AddressResolution.
 Inductive reg_rel_addressing addr_bits : regs_state -> reg_name -> int_mod addr_bits -> int_mod addr_bits -> Prop :=
 | rca_code_pp: forall regs reg reg_val base ofs
                  abs OF_ignored,
-    fetch_gpr regs reg (IntValue reg_val) ->
+    fetch_gpr regs reg = IntValue reg_val ->
     extract_address addr_bits reg_val base ->
     uadd_overflow _ base ofs = (abs, OF_ignored) ->
     reg_rel_addressing addr_bits regs reg ofs abs.
@@ -306,7 +249,7 @@ Inductive fetch_result : Set :=
 Inductive fetch_loc: regs_state -> execution_frame -> mem_manager -> loc -> fetch_result -> Prop :=
 | fetch_reg:
   forall regs ef mm reg_name value,
-    fetch_gpr regs reg_name value ->
+    fetch_gpr regs reg_name = value ->
     fetch_loc regs ef mm (LocReg reg_name) (FetchPV value)
 
 | fetch_imm:
